@prefix rdf: <http://www.w3.org/1999/02/22-rdf-syntax-ns#> .
@prefix rdfs: <http://www.w3.org/2000/01/rdf-schema#> .
@prefix owl: <http://www.w3.org/2002/07/owl#> .
@prefix skos: <http://www.w3.org/2004/02/skos/core#> .
@prefix riskos: <https://w3id.org/risky/riskos#> .
@prefix : <https://w3id.org/risky/riskonto#> .

##############################################################################

: a owl:Ontology ;
    rdfs:label "RiskOnto - Cause"@en .

##############################################################################

# Cause of Risk
:Cause a rdfs:Class, owl:Class ;
    rdfs:label "Cause"@en ;
    rdfs:comment "Indicates a cause or threat that has the potential to materialise associated risk(s)"@en ;
    rdfs:subClassOf :Event .

:RiskMaterialising a rdfs:Class, owl:Class ;
    rdfs:label "Risk Materialising"@en ;
    rdfs:comment "The materialisation of a Cause leading to its potential Risk(s)"@en ;
    rdfs:subClassOf :Event .

:materialisingCause a rdf:Property, owl:ObjectProperty ;
    rdfs:label "materialising cause"@en ;
    rdfs:comment "Indicates cause of materialisation of associated risk(s)"@en ;
    rdfs:domain :RiskMaterialising ;
    rdfs:range :Cause .

:potentialRisk a rdf:Property, owl:ObjectProperty ;
    rdfs:label "potential risk"@en ;
    rdfs:comment "Indicates potential risk that may materialise from associated cause(s)"@en ;
    rdfs:domain :RiskMaterialising ;
    rdfs:range :Risk .

:hasControl a rdf:Property, owl:ObjectProperty ;
    rdfs:label "has control"@en ;
    rdfs:comment "Indicates use of control measure to prevent or reduce risk materialising"@en ;
    rdfs:domain :RiskMaterialising ;
    rdfs:range :ControlMeasure ;
    owl:inverseOf :isControlForRisk .

:isControlForRisk a rdf:Property, owl:ObjectProperty ;
    rdfs:label "is control for risk"@en ;
    rdfs:comment "Indicates the materialising of risk this control affects"@en ;
    rdfs:domain :ControlMeasure ;
    rdfs:range :RiskMaterialising ;
    owl:inverseOf :hasControl .

##############################################################################
