@prefix rdf: <http://www.w3.org/1999/02/22-rdf-syntax-ns#> .
@prefix rdfs: <http://www.w3.org/2000/01/rdf-schema#> .
@prefix owl: <http://www.w3.org/2002/07/owl#> .
@prefix skos: <http://www.w3.org/2004/02/skos/core#> .
@prefix riskos: <https://w3id.org/risky/riskos#> .
@prefix : <https://w3id.org/risky/riskonto#> .

##############################################################################

: a owl:Ontology ;
    rdfs:label "RiskOnto - Consequence"@en .

##############################################################################

# Consequence of Risk
:Consequence a rdfs:Class, owl:Class ;
    rdfs:label "Consequence"@en ;
    rdfs:comment "Indicates a potential consequence materialising from risk(s)"@en ;
    rdfs:subClassOf :Event .

:ConsequenceMaterialising a rdfs:Class, owl:Class ;
    rdfs:label "Consequence Materialising"@en ;
    rdfs:comment "The materialisation of a Risk leading to its potential Consequence(s)"@en ;
    rdfs:subClassOf :Event .

:materialisingRisk a rdf:Property, owl:ObjectProperty ;
    rdfs:label "materialising risk"@en ;
    rdfs:comment "Indicates materialising risk leading to potential consequence(s)"@en ;
    rdfs:domain :ConsequenceMaterialising ;
    rdfs:range :Risk .

:potentialConsequence a rdf:Property, owl:ObjectProperty ;
    rdfs:label "potentialConsequence"@en ;
    rdfs:comment "Indicates potential consequence arising from risk materialising"@en ;
    rdfs:domain :ConsequenceMaterialising ;
    rdfs:range :Consequence .

:hasMitigation a rdf:Property, owl:ObjectProperty ;
    rdfs:label "has mitigation"@en ;
    rdfs:comment "Indicates use of mitigation measure in a Risk-Consequence relationship"@en ;
    rdfs:domain :ConsequenceMaterialising ;
    rdfs:range :MitigationMeasure ;
    owl:inverseOf :isMitigationForConsequenceMaterialising .

:mitigatesConsequence a rdf:Property, owl:ObjectProperty ;
    rdfs:label "mitigates consequence"@en ;
    rdfs:comment "Indicates the materialisation of consequence this mitigation affects"@en ;
    rdfs:domain :MitigationMeasure ;
    rdfs:range :ConsequenceMaterialising ;
    owl:inverseOf :hasMitigation .

##############################################################################
