@prefix rdf: <http://www.w3.org/1999/02/22-rdf-syntax-ns#> .
@prefix rdfs: <http://www.w3.org/2000/01/rdf-schema#> .
@prefix owl: <http://www.w3.org/2002/07/owl#> .
@prefix skos: <http://www.w3.org/2004/02/skos/core#> .
@prefix riskos: <https://w3id.org/risky/riskos#> .
@prefix : <https://w3id.org/risky/riskonto#> .

##############################################################################

: a owl:Ontology ;
    rdfs:label "RiskOnto - Vulnerability"@en .

##############################################################################

# Vulnerability
:Vulnerability a rdfs:Class, owl:Class ;
    rdfs:label "Vulnerability"@en ;
    rdfs:comment "Vulnerability of a Source that can potentially be exploited by threats and/or become a source of risk"@en ;
    rdfs:subClassOf :Event .

:hasVulnerability a rdf:Property, owl:ObjectProperty ;
    rdfs:label "has vulnerability"@en ;
    rdfs:comment "Indicates the risk source has specified vulnerability"@en ;
    rdfs:domain :Source ;
    rdfs:range :Vulnerability ;
    owl:inverseOf :isVulnerabilityOfSource .

:isVulnerabilityOfSource a rdf:Property, owl:ObjectProperty ;
    rdfs:label "is vulnerability of source"@en ;
    rdfs:comment "Indicates the related risk source that has specified vulnerability"@en ;
    rdfs:domain :Vulnerability ;
    rdfs:range :Source ;
    owl:inverseOf :hasVulnerability .

:exploitsVulnerability a rdf:Property, owl:ObjectProperty ;
    rdfs:label "exploits vulnerability"@en ;
    rdfs:comment "Indicates a cause exploits specified vulnerabilities"@en ;
    rdfs:domain :Cause ;
    rdfs:range :Vulnerability ;
    owl:inverseOf :isExploitedIn .

:isExploitedForCause a rdf:Property, owl:ObjectProperty ;
    rdfs:label "is exploited for cause"@en ;
    rdfs:comment "Indicates vulnerability is exploired in specified cause(s)"@en ;
    rdfs:domain :Vulnerability ;
    rdfs:range :Cause ;
    owl:inverseOf :exploitsVulnerability .

:hasSafeguard a rdf:Property, owl:ObjectProperty ;
    rdfs:label "has safeguard"@en ;
    rdfs:comment "Indiciates applicability or existence of safeguard for vulnerability"@en ;
    rdfs:domain :Vulnerability ;
    rdfs:range :Safeguard ;
    owl:inverseOf :safeguardsAgainstVulnerability .

:safeguardsAgainstVulnerability a rdf:Property, owl:ObjectProperty ;
    rdfs:label "safeguards against vulnerability"@en ;
    rdfs:comment "Indiciates applicability of safeguard for specified vulnerability"@en ;
    rdfs:domain :Safeguard ;
    rdfs:range :Vulnerability ;
    owl:inverseOf :hasSafeguard .
    
##############################################################################