@prefix rdf: <http://www.w3.org/1999/02/22-rdf-syntax-ns#> .
@prefix rdfs: <http://www.w3.org/2000/01/rdf-schema#> .
@prefix owl: <http://www.w3.org/2002/07/owl#> .
@prefix skos: <http://www.w3.org/2004/02/skos/core#> .
@prefix riskos: <https://w3id.org/risky/riskos#> .
@prefix : <https://w3id.org/risky/riskonto#> .

##############################################################################

: a owl:Ontology ;
    rdfs:label "RiskOnto"@en .

##############################################################################

# Risk
:Risk a rdfs:Class, owl:Class ;
    rdfs:label "Risk"@en ;
    rdfs:subClassOf :Event .

# Source of Risk
:Source a rdfs:Class, owl:Class ;
    rdfs:label "Source"@en ;
    rdfs:comment "Indicates the source of risk i.e. the risk exists because of the source"@en .

:hasRisk a rdf:Property, owl:ObjectProperty ;
    rdfs:label "has risk"@en ;
    rdfs:comment "Indicates a source has a risk associated with it"@en ;
    rdfs:domain :Source ;
    rdfs:range :Risk ;
    owl:inverseOf :hasSource .

:hasSource a rdf:Property, owl:ObjectProperty ;
    rdfs:label "has source"@en ;
    rdfs:comment "Indicates a risk has a source associated with it"@en ;
    rdfs:domain :Risk ;
    rdfs:range :Source ;
    owl:inverseOf :isSourceForRisk .

##############################################################################

# Measures
:Measure a rdfs:Class, owl:Class ;
    rdfs:label "Measure"@en ;
    rdfs:comment "A measure is intended to change, modifiy, or remove the probability, likelihood, or severity of an event"@en .

:ControlMeasure a rdfs:Class, owl:Class ;
    rdfs:label "Control Measure"@en ;
    rdfs:comment "A control is a measure intended to reduce the probability, likelihood, or severity of a cause with potential for risk"@en ;
    rdfs:subClassOf :Measure .

:MitigationMeasure a rdfs:Class, owl:Class ;
    rdfs:label "Mitigation Measure"@en ;
    rdfs:comment "A mitigation is a measure intended to reduce the probability, likelihood, or severity of a potential consequence resulting from risk"@en ;
    rdfs:subClassOf :Measure .

:Safeguard a rdfs:Class, owl:Class ;
    rdfs:label "Safegard"@en ;
    rdfs:comment "A safeguard is a measure for reducing the vulnerability and/or its exploitation"@en ;
    rdfs:subClassOf :Measure .

##############################################################################

# Cause of Risk
:Cause a rdfs:Class, owl:Class ;
    rdfs:label "Cause"@en ;
    rdfs:comment "Indicates a cause or threat that has the potential to materialise associated risk(s)"@en ;
    rdfs:subClassOf :Event .

:RiskMaterialising a rdfs:Class, owl:Class ;
    rdfs:label "Risk Materialising"@en ;
    rdfs:comment "The materialisation of a Cause leading to its potential Risk(s)"@en ;
    rdfs:subClassOf :Event .

:materialisingCause a rdf:Property, owl:ObjectProperty ;
    rdfs:label "materialising cause"@en ;
    rdfs:comment "Indicates cause of materialisation of associated risk(s)"@en ;
    rdfs:domain :RiskMaterialising ;
    rdfs:range :Cause .

:potentialRisk a rdf:Property, owl:ObjectProperty ;
    rdfs:label "potential risk"@en ;
    rdfs:comment "Indicates potential risk that may materialise from associated cause(s)"@en ;
    rdfs:domain :RiskMaterialising ;
    rdfs:range :Risk .

:hasControl a rdf:Property, owl:ObjectProperty ;
    rdfs:label "has control"@en ;
    rdfs:comment "Indicates use of control measure to prevent or reduce risk materialising"@en ;
    rdfs:domain :RiskMaterialising ;
    rdfs:range :ControlMeasure ;
    owl:inverseOf :isControlForRisk .

:isControlForRisk a rdf:Property, owl:ObjectProperty ;
    rdfs:label "is control for risk"@en ;
    rdfs:comment "Indicates the materialising of risk this control affects"@en ;
    rdfs:domain :ControlMeasure ;
    rdfs:range :RiskMaterialising ;
    owl:inverseOf :hasControl .

##############################################################################

# Consequence of Risk
:Consequence a rdfs:Class, owl:Class ;
    rdfs:label "Consequence"@en ;
    rdfs:comment "Indicates a potential consequence materialising from risk(s)"@en ;
    rdfs:subClassOf :Event .

:ConsequenceMaterialising a rdfs:Class, owl:Class ;
    rdfs:label "Consequence Materialising"@en ;
    rdfs:comment "The materialisation of a Risk leading to its potential Consequence(s)"@en ;
    rdfs:subClassOf :Event .

:materialisingRisk a rdf:Property, owl:ObjectProperty ;
    rdfs:label "materialising risk"@en ;
    rdfs:comment "Indicates materialising risk leading to potential consequence(s)"@en ;
    rdfs:domain :ConsequenceMaterialising ;
    rdfs:range :Risk .

:potentialConsequence a rdf:Property, owl:ObjectProperty ;
    rdfs:label "potentialConsequence"@en ;
    rdfs:comment "Indicates potential consequence arising from risk materialising"@en ;
    rdfs:domain :ConsequenceMaterialising ;
    rdfs:range :Consequence .

:hasMitigation a rdf:Property, owl:ObjectProperty ;
    rdfs:label "has mitigation"@en ;
    rdfs:comment "Indicates use of mitigation measure in a Risk-Consequence relationship"@en ;
    rdfs:domain :ConsequenceMaterialising ;
    rdfs:range :MitigationMeasure ;
    owl:inverseOf :isMitigationForConsequenceMaterialising .

:mitigatesConsequence a rdf:Property, owl:ObjectProperty ;
    rdfs:label "mitigates consequence"@en ;
    rdfs:comment "Indicates the materialisation of consequence this mitigation affects"@en ;
    rdfs:domain :MitigationMeasure ;
    rdfs:range :ConsequenceMaterialising ;
    owl:inverseOf :hasMitigation .

##############################################################################

# Impact of Consequence
:Impact a rdfs:Class, owl:Class ;
    rdfs:label "Impact"@en ;
    rdfs:comment "Indicates potential impact(s) arising from consequence(s)"@en ;
    rdfs:subClassOf :Consequence .

:ImpactMaterialising a rdfs:Class, owl:Class ;
    rdfs:label "Impact Materialising"@en ;
    rdfs:comment "The materialisation of a Consequence leading to its potential Impact(s)"@en ;
    rdfs:subClassOf :Event .

:materialisingConsequence a rdf:Property, owl:ObjectProperty ;
    rdfs:label "materialising consequence"@en ;
    rdfs:comment "Indicates the materialising consenquence causing potential imapct(s)"@en ;
    rdfs:domain :ImpactMaterialising ;
    rdfs:range :Consequence .

:potentialImpact a rdf:Property, owl:ObjectProperty ;
    rdfs:label "potential impact"@en ;
    rdfs:comment "Indicates the potential impact arising from materialising consequence(s)"@en ;
    rdfs:domain :ImpactMaterialising ;
    rdfs:range :Impact .

:effectOfImpact a rdf:Property, owl:ObjectProperty ;
    rdfs:label "effect of impact"@en ;
    rdfs:comment "Indicates effects of impact and the affected things, stakeholders, or events"@en ;
    rdfs:domain :Impact ;
    rdfs:range rdfs:Resource .

##############################################################################

# Vulnerability
:Vulnerability a rdfs:Class, owl:Class ;
    rdfs:label "Vulnerability"@en ;
    rdfs:comment "Vulnerability of a Source that can potentially be exploited by threats and/or become a source of risk"@en ;
    rdfs:subClassOf :Event .

:hasVulnerability a rdf:Property, owl:ObjectProperty ;
    rdfs:label "has vulnerability"@en ;
    rdfs:comment "Indicates the risk source has specified vulnerability"@en ;
    rdfs:domain :Source ;
    rdfs:range :Vulnerability ;
    owl:inverseOf :isVulnerabilityOfSource .

:isVulnerabilityOfSource a rdf:Property, owl:ObjectProperty ;
    rdfs:label "is vulnerability of source"@en ;
    rdfs:comment "Indicates the related risk source that has specified vulnerability"@en ;
    rdfs:domain :Vulnerability ;
    rdfs:range :Source ;
    owl:inverseOf :hasVulnerability .

:exploitsVulnerability a rdf:Property, owl:ObjectProperty ;
    rdfs:label "exploits vulnerability"@en ;
    rdfs:comment "Indicates a cause exploits specified vulnerabilities"@en ;
    rdfs:domain :Cause ;
    rdfs:range :Vulnerability ;
    owl:inverseOf :isExploitedIn .

:isExploitedForCause a rdf:Property, owl:ObjectProperty ;
    rdfs:label "is exploited for cause"@en ;
    rdfs:comment "Indicates vulnerability is exploired in specified cause(s)"@en ;
    rdfs:domain :Vulnerability ;
    rdfs:range :Cause ;
    owl:inverseOf :exploitsVulnerability .

:hasSafeguard a rdf:Property, owl:ObjectProperty ;
    rdfs:label "has safeguard"@en ;
    rdfs:comment "Indiciates applicability or existence of safeguard for vulnerability"@en ;
    rdfs:domain :Vulnerability ;
    rdfs:range :Safeguard ;
    owl:inverseOf :safeguardsAgainstVulnerability .

:safeguardsAgainstVulnerability a rdf:Property, owl:ObjectProperty ;
    rdfs:label "safeguards against vulnerability"@en ;
    rdfs:comment "Indiciates applicability of safeguard for specified vulnerability"@en ;
    rdfs:domain :Safeguard ;
    rdfs:range :Vulnerability ;
    owl:inverseOf :hasSafeguard .

##############################################################################