@prefix : <https://w3id.org/dpv/risk/matrix#> .

:RiskMatrixLevel a skos:Concept ;
    skos:prefLabel "Risk Matrix Level"@en ;
    skos:definition "Risk Level as expressed as a combination of Severity and Likelihood within a Risk Matrix"@en ;
    skos:broader :RiskLevel .

:RiskMatrix3x3 a skos:Concept ;
    skos:prefLabel "Risk Matrix 3x3"@en ;
    skos:definition "A Risk Matrix with 3 Risk Levels, 3 Severity levels, and 3 Likelihood levels"@en ;
    skos:broader :RiskMatrix .
:RiskMatrix5x5 a skos:Concept ;
    skos:prefLabel "Risk Matrix 5x5"@en ;
    skos:definition "A Risk Matrix with 5 Risk Levels, 5 Severity levels, and 5 Likelihood levels"@en ;
    skos:broader :RiskMatrix .
:RiskMatrix7x7 a skos:Concept ;
    skos:prefLabel "Risk Matrix 7x7"@en ;
    skos:definition "A Risk Matrix with 7 Risk Levels, 7 Severity levels, and 7 Likelihood levels"@en ;
    skos:broader :RiskMatrix .

# Template for N x N matrix
#:RM{N}x{N}N1 a skos:Concept ;
#    skos:prefLabel "{LABEL}"@en ;
#    dpv:hasRiskLevel :{RiskLevel} ;
#    dpv:hasSeverity :{SeverityLevel} ;
#    dpv:hasLikelihood :{LikelihoodLevel} ;
#    skos:broader :RiskMatrix{N}x{N} .

# ----- AUTOGENERATED CONTENT -----

:RM3x3R1C1 a skos:Concept ;
    skos:broader :RiskMatrix3x3 ;
    skos:definition "Node (row: 1, col: 1) in 3x3 risk matrix with risk level 0, severity Low, and likelihood Low"@en ;
    skos:prefLabel "Low Risk"@en ;
    dpv:hasLikelihood :LowLikelihood ;
    dpv:hasRiskLevel :LowRisk ;
    dpv:hasSeverity :LowSeverity .

:RM3x3R1C2 a skos:Concept ;
    skos:broader :RiskMatrix3x3 ;
    skos:definition "Node (row: 1, col: 2) in 3x3 risk matrix with risk level 0, severity Moderate, and likelihood Low"@en ;
    skos:prefLabel "Low Risk"@en ;
    dpv:hasLikelihood :LowLikelihood ;
    dpv:hasRiskLevel :LowRisk ;
    dpv:hasSeverity :ModerateSeverity .

:RM3x3R1C3 a skos:Concept ;
    skos:broader :RiskMatrix3x3 ;
    skos:definition "Node (row: 1, col: 3) in 3x3 risk matrix with risk level 1, severity High, and likelihood Low"@en ;
    skos:prefLabel "Moderate Risk"@en ;
    dpv:hasLikelihood :LowLikelihood ;
    dpv:hasRiskLevel :ModerateRisk ;
    dpv:hasSeverity :HighSeverity .

:RM3x3R2C1 a skos:Concept ;
    skos:broader :RiskMatrix3x3 ;
    skos:definition "Node (row: 2, col: 1) in 3x3 risk matrix with risk level 0, severity Low, and likelihood Moderate"@en ;
    skos:prefLabel "Low Risk"@en ;
    dpv:hasLikelihood :ModerateLikelihood ;
    dpv:hasRiskLevel :LowRisk ;
    dpv:hasSeverity :LowSeverity .

:RM3x3R2C2 a skos:Concept ;
    skos:broader :RiskMatrix3x3 ;
    skos:definition "Node (row: 2, col: 2) in 3x3 risk matrix with risk level 1, severity Moderate, and likelihood Moderate"@en ;
    skos:prefLabel "Moderate Risk"@en ;
    dpv:hasLikelihood :ModerateLikelihood ;
    dpv:hasRiskLevel :ModerateRisk ;
    dpv:hasSeverity :ModerateSeverity .

:RM3x3R2C3 a skos:Concept ;
    skos:broader :RiskMatrix3x3 ;
    skos:definition "Node (row: 2, col: 3) in 3x3 risk matrix with risk level 2, severity High, and likelihood Moderate"@en ;
    skos:prefLabel "High Risk"@en ;
    dpv:hasLikelihood :ModerateLikelihood ;
    dpv:hasRiskLevel :HighRisk ;
    dpv:hasSeverity :HighSeverity .

:RM3x3R3C1 a skos:Concept ;
    skos:broader :RiskMatrix3x3 ;
    skos:definition "Node (row: 3, col: 1) in 3x3 risk matrix with risk level 1, severity Low, and likelihood High"@en ;
    skos:prefLabel "Moderate Risk"@en ;
    dpv:hasLikelihood :HighLikelihood ;
    dpv:hasRiskLevel :ModerateRisk ;
    dpv:hasSeverity :LowSeverity .

:RM3x3R3C2 a skos:Concept ;
    skos:broader :RiskMatrix3x3 ;
    skos:definition "Node (row: 3, col: 2) in 3x3 risk matrix with risk level 2, severity Moderate, and likelihood High"@en ;
    skos:prefLabel "High Risk"@en ;
    dpv:hasLikelihood :HighLikelihood ;
    dpv:hasRiskLevel :HighRisk ;
    dpv:hasSeverity :ModerateSeverity .

:RM3x3R3C3 a skos:Concept ;
    skos:broader :RiskMatrix3x3 ;
    skos:definition "Node (row: 3, col: 3) in 3x3 risk matrix with risk level 2, severity High, and likelihood High"@en ;
    skos:prefLabel "High Risk"@en ;
    dpv:hasLikelihood :HighLikelihood ;
    dpv:hasRiskLevel :HighRisk ;
    dpv:hasSeverity :HighSeverity .

:RM5x5R1C1 a skos:Concept ;
    skos:broader :RiskMatrix5x5 ;
    skos:definition "Node (row: 1, col: 1) in 5x5 risk matrix with risk level 0, severity VeryLow, and likelihood VeryLow"@en ;
    skos:prefLabel "Very Low Risk"@en ;
    dpv:hasLikelihood :VeryLowLikelihood ;
    dpv:hasRiskLevel :VeryLowRisk ;
    dpv:hasSeverity :VeryLowSeverity .

:RM5x5R1C2 a skos:Concept ;
    skos:broader :RiskMatrix5x5 ;
    skos:definition "Node (row: 1, col: 2) in 5x5 risk matrix with risk level 0, severity Low, and likelihood VeryLow"@en ;
    skos:prefLabel "Very Low Risk"@en ;
    dpv:hasLikelihood :VeryLowLikelihood ;
    dpv:hasRiskLevel :VeryLowRisk ;
    dpv:hasSeverity :LowSeverity .

:RM5x5R1C3 a skos:Concept ;
    skos:broader :RiskMatrix5x5 ;
    skos:definition "Node (row: 1, col: 3) in 5x5 risk matrix with risk level 0, severity Moderate, and likelihood VeryLow"@en ;
    skos:prefLabel "Very Low Risk"@en ;
    dpv:hasLikelihood :VeryLowLikelihood ;
    dpv:hasRiskLevel :VeryLowRisk ;
    dpv:hasSeverity :ModerateSeverity .

:RM5x5R1C4 a skos:Concept ;
    skos:broader :RiskMatrix5x5 ;
    skos:definition "Node (row: 1, col: 4) in 5x5 risk matrix with risk level 1, severity High, and likelihood VeryLow"@en ;
    skos:prefLabel "Low Risk"@en ;
    dpv:hasLikelihood :VeryLowLikelihood ;
    dpv:hasRiskLevel :LowRisk ;
    dpv:hasSeverity :HighSeverity .

:RM5x5R1C5 a skos:Concept ;
    skos:broader :RiskMatrix5x5 ;
    skos:definition "Node (row: 1, col: 5) in 5x5 risk matrix with risk level 1, severity VeryHigh, and likelihood VeryLow"@en ;
    skos:prefLabel "Low Risk"@en ;
    dpv:hasLikelihood :VeryLowLikelihood ;
    dpv:hasRiskLevel :LowRisk ;
    dpv:hasSeverity :VeryHighSeverity .

:RM5x5R2C1 a skos:Concept ;
    skos:broader :RiskMatrix5x5 ;
    skos:definition "Node (row: 2, col: 1) in 5x5 risk matrix with risk level 0, severity VeryLow, and likelihood Low"@en ;
    skos:prefLabel "Very Low Risk"@en ;
    dpv:hasLikelihood :LowLikelihood ;
    dpv:hasRiskLevel :VeryLowRisk ;
    dpv:hasSeverity :VeryLowSeverity .

:RM5x5R2C2 a skos:Concept ;
    skos:broader :RiskMatrix5x5 ;
    skos:definition "Node (row: 2, col: 2) in 5x5 risk matrix with risk level 1, severity Low, and likelihood Low"@en ;
    skos:prefLabel "Low Risk"@en ;
    dpv:hasLikelihood :LowLikelihood ;
    dpv:hasRiskLevel :LowRisk ;
    dpv:hasSeverity :LowSeverity .

:RM5x5R2C3 a skos:Concept ;
    skos:broader :RiskMatrix5x5 ;
    skos:definition "Node (row: 2, col: 3) in 5x5 risk matrix with risk level 2, severity Moderate, and likelihood Low"@en ;
    skos:prefLabel "Moderate Risk"@en ;
    dpv:hasLikelihood :LowLikelihood ;
    dpv:hasRiskLevel :ModerateRisk ;
    dpv:hasSeverity :ModerateSeverity .

:RM5x5R2C4 a skos:Concept ;
    skos:broader :RiskMatrix5x5 ;
    skos:definition "Node (row: 2, col: 4) in 5x5 risk matrix with risk level 2, severity High, and likelihood Low"@en ;
    skos:prefLabel "Moderate Risk"@en ;
    dpv:hasLikelihood :LowLikelihood ;
    dpv:hasRiskLevel :ModerateRisk ;
    dpv:hasSeverity :HighSeverity .

:RM5x5R2C5 a skos:Concept ;
    skos:broader :RiskMatrix5x5 ;
    skos:definition "Node (row: 2, col: 5) in 5x5 risk matrix with risk level 3, severity VeryHigh, and likelihood Low"@en ;
    skos:prefLabel "High Risk"@en ;
    dpv:hasLikelihood :LowLikelihood ;
    dpv:hasRiskLevel :HighRisk ;
    dpv:hasSeverity :VeryHighSeverity .

:RM5x5R3C1 a skos:Concept ;
    skos:broader :RiskMatrix5x5 ;
    skos:definition "Node (row: 3, col: 1) in 5x5 risk matrix with risk level 0, severity VeryLow, and likelihood Moderate"@en ;
    skos:prefLabel "Very Low Risk"@en ;
    dpv:hasLikelihood :ModerateLikelihood ;
    dpv:hasRiskLevel :VeryLowRisk ;
    dpv:hasSeverity :VeryLowSeverity .

:RM5x5R3C2 a skos:Concept ;
    skos:broader :RiskMatrix5x5 ;
    skos:definition "Node (row: 3, col: 2) in 5x5 risk matrix with risk level 2, severity Low, and likelihood Moderate"@en ;
    skos:prefLabel "Moderate Risk"@en ;
    dpv:hasLikelihood :ModerateLikelihood ;
    dpv:hasRiskLevel :ModerateRisk ;
    dpv:hasSeverity :LowSeverity .

:RM5x5R3C3 a skos:Concept ;
    skos:broader :RiskMatrix5x5 ;
    skos:definition "Node (row: 3, col: 3) in 5x5 risk matrix with risk level 2, severity Moderate, and likelihood Moderate"@en ;
    skos:prefLabel "Moderate Risk"@en ;
    dpv:hasLikelihood :ModerateLikelihood ;
    dpv:hasRiskLevel :ModerateRisk ;
    dpv:hasSeverity :ModerateSeverity .

:RM5x5R3C4 a skos:Concept ;
    skos:broader :RiskMatrix5x5 ;
    skos:definition "Node (row: 3, col: 4) in 5x5 risk matrix with risk level 3, severity High, and likelihood Moderate"@en ;
    skos:prefLabel "High Risk"@en ;
    dpv:hasLikelihood :ModerateLikelihood ;
    dpv:hasRiskLevel :HighRisk ;
    dpv:hasSeverity :HighSeverity .

:RM5x5R3C5 a skos:Concept ;
    skos:broader :RiskMatrix5x5 ;
    skos:definition "Node (row: 3, col: 5) in 5x5 risk matrix with risk level 3, severity VeryHigh, and likelihood Moderate"@en ;
    skos:prefLabel "High Risk"@en ;
    dpv:hasLikelihood :ModerateLikelihood ;
    dpv:hasRiskLevel :HighRisk ;
    dpv:hasSeverity :VeryHighSeverity .

:RM5x5R4C1 a skos:Concept ;
    skos:broader :RiskMatrix5x5 ;
    skos:definition "Node (row: 4, col: 1) in 5x5 risk matrix with risk level 1, severity VeryLow, and likelihood High"@en ;
    skos:prefLabel "Low Risk"@en ;
    dpv:hasLikelihood :HighLikelihood ;
    dpv:hasRiskLevel :LowRisk ;
    dpv:hasSeverity :VeryLowSeverity .

:RM5x5R4C2 a skos:Concept ;
    skos:broader :RiskMatrix5x5 ;
    skos:definition "Node (row: 4, col: 2) in 5x5 risk matrix with risk level 2, severity Low, and likelihood High"@en ;
    skos:prefLabel "Moderate Risk"@en ;
    dpv:hasLikelihood :HighLikelihood ;
    dpv:hasRiskLevel :ModerateRisk ;
    dpv:hasSeverity :LowSeverity .

:RM5x5R4C3 a skos:Concept ;
    skos:broader :RiskMatrix5x5 ;
    skos:definition "Node (row: 4, col: 3) in 5x5 risk matrix with risk level 3, severity Moderate, and likelihood High"@en ;
    skos:prefLabel "High Risk"@en ;
    dpv:hasLikelihood :HighLikelihood ;
    dpv:hasRiskLevel :HighRisk ;
    dpv:hasSeverity :ModerateSeverity .

:RM5x5R4C4 a skos:Concept ;
    skos:broader :RiskMatrix5x5 ;
    skos:definition "Node (row: 4, col: 4) in 5x5 risk matrix with risk level 4, severity High, and likelihood High"@en ;
    skos:prefLabel "Very High Risk"@en ;
    dpv:hasLikelihood :HighLikelihood ;
    dpv:hasRiskLevel :VeryHighRisk ;
    dpv:hasSeverity :HighSeverity .

:RM5x5R4C5 a skos:Concept ;
    skos:broader :RiskMatrix5x5 ;
    skos:definition "Node (row: 4, col: 5) in 5x5 risk matrix with risk level 4, severity VeryHigh, and likelihood High"@en ;
    skos:prefLabel "Very High Risk"@en ;
    dpv:hasLikelihood :HighLikelihood ;
    dpv:hasRiskLevel :VeryHighRisk ;
    dpv:hasSeverity :VeryHighSeverity .

:RM5x5R5C1 a skos:Concept ;
    skos:broader :RiskMatrix5x5 ;
    skos:definition "Node (row: 5, col: 1) in 5x5 risk matrix with risk level 1, severity VeryLow, and likelihood VeryHigh"@en ;
    skos:prefLabel "Low Risk"@en ;
    dpv:hasLikelihood :VeryHighLikelihood ;
    dpv:hasRiskLevel :LowRisk ;
    dpv:hasSeverity :VeryLowSeverity .

:RM5x5R5C2 a skos:Concept ;
    skos:broader :RiskMatrix5x5 ;
    skos:definition "Node (row: 5, col: 2) in 5x5 risk matrix with risk level 3, severity Low, and likelihood VeryHigh"@en ;
    skos:prefLabel "High Risk"@en ;
    dpv:hasLikelihood :VeryHighLikelihood ;
    dpv:hasRiskLevel :HighRisk ;
    dpv:hasSeverity :LowSeverity .

:RM5x5R5C3 a skos:Concept ;
    skos:broader :RiskMatrix5x5 ;
    skos:definition "Node (row: 5, col: 3) in 5x5 risk matrix with risk level 4, severity Moderate, and likelihood VeryHigh"@en ;
    skos:prefLabel "Very High Risk"@en ;
    dpv:hasLikelihood :VeryHighLikelihood ;
    dpv:hasRiskLevel :VeryHighRisk ;
    dpv:hasSeverity :ModerateSeverity .

:RM5x5R5C4 a skos:Concept ;
    skos:broader :RiskMatrix5x5 ;
    skos:definition "Node (row: 5, col: 4) in 5x5 risk matrix with risk level 4, severity High, and likelihood VeryHigh"@en ;
    skos:prefLabel "Very High Risk"@en ;
    dpv:hasLikelihood :VeryHighLikelihood ;
    dpv:hasRiskLevel :VeryHighRisk ;
    dpv:hasSeverity :HighSeverity .

:RM5x5R5C5 a skos:Concept ;
    skos:broader :RiskMatrix5x5 ;
    skos:definition "Node (row: 5, col: 5) in 5x5 risk matrix with risk level 4, severity VeryHigh, and likelihood VeryHigh"@en ;
    skos:prefLabel "Very High Risk"@en ;
    dpv:hasLikelihood :VeryHighLikelihood ;
    dpv:hasRiskLevel :VeryHighRisk ;
    dpv:hasSeverity :VeryHighSeverity .

:RM7x7R1C1 a skos:Concept ;
    skos:broader :RiskMatrix7x7 ;
    skos:definition "Node (row: 1, col: 1) in 7x7 risk matrix with risk level 0, severity ExtremelyLow, and likelihood ExtremelyLow"@en ;
    skos:prefLabel "Extremely Low Risk"@en ;
    dpv:hasLikelihood :ExtremelyLowLikelihood ;
    dpv:hasRiskLevel :ExtremelyLowRisk ;
    dpv:hasSeverity :ExtremelyLowSeverity .

:RM7x7R1C2 a skos:Concept ;
    skos:broader :RiskMatrix7x7 ;
    skos:definition "Node (row: 1, col: 2) in 7x7 risk matrix with risk level 0, severity VeryLow, and likelihood ExtremelyLow"@en ;
    skos:prefLabel "Extremely Low Risk"@en ;
    dpv:hasLikelihood :ExtremelyLowLikelihood ;
    dpv:hasRiskLevel :ExtremelyLowRisk ;
    dpv:hasSeverity :VeryLowSeverity .

:RM7x7R1C3 a skos:Concept ;
    skos:broader :RiskMatrix7x7 ;
    skos:definition "Node (row: 1, col: 3) in 7x7 risk matrix with risk level 0, severity Low, and likelihood ExtremelyLow"@en ;
    skos:prefLabel "Extremely Low Risk"@en ;
    dpv:hasLikelihood :ExtremelyLowLikelihood ;
    dpv:hasRiskLevel :ExtremelyLowRisk ;
    dpv:hasSeverity :LowSeverity .

:RM7x7R1C4 a skos:Concept ;
    skos:broader :RiskMatrix7x7 ;
    skos:definition "Node (row: 1, col: 4) in 7x7 risk matrix with risk level 0, severity Moderate, and likelihood ExtremelyLow"@en ;
    skos:prefLabel "Extremely Low Risk"@en ;
    dpv:hasLikelihood :ExtremelyLowLikelihood ;
    dpv:hasRiskLevel :ExtremelyLowRisk ;
    dpv:hasSeverity :ModerateSeverity .

:RM7x7R1C5 a skos:Concept ;
    skos:broader :RiskMatrix7x7 ;
    skos:definition "Node (row: 1, col: 5) in 7x7 risk matrix with risk level 1, severity High, and likelihood ExtremelyLow"@en ;
    skos:prefLabel "Very Low Risk"@en ;
    dpv:hasLikelihood :ExtremelyLowLikelihood ;
    dpv:hasRiskLevel :VeryLowRisk ;
    dpv:hasSeverity :HighSeverity .

:RM7x7R1C6 a skos:Concept ;
    skos:broader :RiskMatrix7x7 ;
    skos:definition "Node (row: 1, col: 6) in 7x7 risk matrix with risk level 1, severity VeryHigh, and likelihood ExtremelyLow"@en ;
    skos:prefLabel "Very Low Risk"@en ;
    dpv:hasLikelihood :ExtremelyLowLikelihood ;
    dpv:hasRiskLevel :VeryLowRisk ;
    dpv:hasSeverity :VeryHighSeverity .

:RM7x7R1C7 a skos:Concept ;
    skos:broader :RiskMatrix7x7 ;
    skos:definition "Node (row: 1, col: 7) in 7x7 risk matrix with risk level 2, severity ExtremelyHigh, and likelihood ExtremelyLow"@en ;
    skos:prefLabel "Low Risk"@en ;
    dpv:hasLikelihood :ExtremelyLowLikelihood ;
    dpv:hasRiskLevel :LowRisk ;
    dpv:hasSeverity :ExtremelyHighSeverity .

:RM7x7R2C1 a skos:Concept ;
    skos:broader :RiskMatrix7x7 ;
    skos:definition "Node (row: 2, col: 1) in 7x7 risk matrix with risk level 0, severity ExtremelyLow, and likelihood VeryLow"@en ;
    skos:prefLabel "Extremely Low Risk"@en ;
    dpv:hasLikelihood :VeryLowLikelihood ;
    dpv:hasRiskLevel :ExtremelyLowRisk ;
    dpv:hasSeverity :ExtremelyLowSeverity .

:RM7x7R2C2 a skos:Concept ;
    skos:broader :RiskMatrix7x7 ;
    skos:definition "Node (row: 2, col: 2) in 7x7 risk matrix with risk level 0, severity VeryLow, and likelihood VeryLow"@en ;
    skos:prefLabel "Extremely Low Risk"@en ;
    dpv:hasLikelihood :VeryLowLikelihood ;
    dpv:hasRiskLevel :ExtremelyLowRisk ;
    dpv:hasSeverity :VeryLowSeverity .

:RM7x7R2C3 a skos:Concept ;
    skos:broader :RiskMatrix7x7 ;
    skos:definition "Node (row: 2, col: 3) in 7x7 risk matrix with risk level 1, severity Low, and likelihood VeryLow"@en ;
    skos:prefLabel "Very Low Risk"@en ;
    dpv:hasLikelihood :VeryLowLikelihood ;
    dpv:hasRiskLevel :VeryLowRisk ;
    dpv:hasSeverity :LowSeverity .

:RM7x7R2C4 a skos:Concept ;
    skos:broader :RiskMatrix7x7 ;
    skos:definition "Node (row: 2, col: 4) in 7x7 risk matrix with risk level 2, severity Moderate, and likelihood VeryLow"@en ;
    skos:prefLabel "Low Risk"@en ;
    dpv:hasLikelihood :VeryLowLikelihood ;
    dpv:hasRiskLevel :LowRisk ;
    dpv:hasSeverity :ModerateSeverity .

:RM7x7R2C5 a skos:Concept ;
    skos:broader :RiskMatrix7x7 ;
    skos:definition "Node (row: 2, col: 5) in 7x7 risk matrix with risk level 2, severity High, and likelihood VeryLow"@en ;
    skos:prefLabel "Low Risk"@en ;
    dpv:hasLikelihood :VeryLowLikelihood ;
    dpv:hasRiskLevel :LowRisk ;
    dpv:hasSeverity :HighSeverity .

:RM7x7R2C6 a skos:Concept ;
    skos:broader :RiskMatrix7x7 ;
    skos:definition "Node (row: 2, col: 6) in 7x7 risk matrix with risk level 3, severity VeryHigh, and likelihood VeryLow"@en ;
    skos:prefLabel "Moderate Risk"@en ;
    dpv:hasLikelihood :VeryLowLikelihood ;
    dpv:hasRiskLevel :ModerateRisk ;
    dpv:hasSeverity :VeryHighSeverity .

:RM7x7R2C7 a skos:Concept ;
    skos:broader :RiskMatrix7x7 ;
    skos:definition "Node (row: 2, col: 7) in 7x7 risk matrix with risk level 3, severity ExtremelyHigh, and likelihood VeryLow"@en ;
    skos:prefLabel "Moderate Risk"@en ;
    dpv:hasLikelihood :VeryLowLikelihood ;
    dpv:hasRiskLevel :ModerateRisk ;
    dpv:hasSeverity :ExtremelyHighSeverity .

:RM7x7R3C1 a skos:Concept ;
    skos:broader :RiskMatrix7x7 ;
    skos:definition "Node (row: 3, col: 1) in 7x7 risk matrix with risk level 0, severity ExtremelyLow, and likelihood Low"@en ;
    skos:prefLabel "Extremely Low Risk"@en ;
    dpv:hasLikelihood :LowLikelihood ;
    dpv:hasRiskLevel :ExtremelyLowRisk ;
    dpv:hasSeverity :ExtremelyLowSeverity .

:RM7x7R3C2 a skos:Concept ;
    skos:broader :RiskMatrix7x7 ;
    skos:definition "Node (row: 3, col: 2) in 7x7 risk matrix with risk level 1, severity VeryLow, and likelihood Low"@en ;
    skos:prefLabel "Very Low Risk"@en ;
    dpv:hasLikelihood :LowLikelihood ;
    dpv:hasRiskLevel :VeryLowRisk ;
    dpv:hasSeverity :VeryLowSeverity .

:RM7x7R3C3 a skos:Concept ;
    skos:broader :RiskMatrix7x7 ;
    skos:definition "Node (row: 3, col: 3) in 7x7 risk matrix with risk level 2, severity Low, and likelihood Low"@en ;
    skos:prefLabel "Low Risk"@en ;
    dpv:hasLikelihood :LowLikelihood ;
    dpv:hasRiskLevel :LowRisk ;
    dpv:hasSeverity :LowSeverity .

:RM7x7R3C4 a skos:Concept ;
    skos:broader :RiskMatrix7x7 ;
    skos:definition "Node (row: 3, col: 4) in 7x7 risk matrix with risk level 3, severity Moderate, and likelihood Low"@en ;
    skos:prefLabel "Moderate Risk"@en ;
    dpv:hasLikelihood :LowLikelihood ;
    dpv:hasRiskLevel :ModerateRisk ;
    dpv:hasSeverity :ModerateSeverity .

:RM7x7R3C5 a skos:Concept ;
    skos:broader :RiskMatrix7x7 ;
    skos:definition "Node (row: 3, col: 5) in 7x7 risk matrix with risk level 3, severity High, and likelihood Low"@en ;
    skos:prefLabel "Moderate Risk"@en ;
    dpv:hasLikelihood :LowLikelihood ;
    dpv:hasRiskLevel :ModerateRisk ;
    dpv:hasSeverity :HighSeverity .

:RM7x7R3C6 a skos:Concept ;
    skos:broader :RiskMatrix7x7 ;
    skos:definition "Node (row: 3, col: 6) in 7x7 risk matrix with risk level 4, severity VeryHigh, and likelihood Low"@en ;
    skos:prefLabel "High Risk"@en ;
    dpv:hasLikelihood :LowLikelihood ;
    dpv:hasRiskLevel :HighRisk ;
    dpv:hasSeverity :VeryHighSeverity .

:RM7x7R3C7 a skos:Concept ;
    skos:broader :RiskMatrix7x7 ;
    skos:definition "Node (row: 3, col: 7) in 7x7 risk matrix with risk level 4, severity ExtremelyHigh, and likelihood Low"@en ;
    skos:prefLabel "High Risk"@en ;
    dpv:hasLikelihood :LowLikelihood ;
    dpv:hasRiskLevel :HighRisk ;
    dpv:hasSeverity :ExtremelyHighSeverity .

:RM7x7R4C1 a skos:Concept ;
    skos:broader :RiskMatrix7x7 ;
    skos:definition "Node (row: 4, col: 1) in 7x7 risk matrix with risk level 1, severity ExtremelyLow, and likelihood Moderate"@en ;
    skos:prefLabel "Very Low Risk"@en ;
    dpv:hasLikelihood :ModerateLikelihood ;
    dpv:hasRiskLevel :VeryLowRisk ;
    dpv:hasSeverity :ExtremelyLowSeverity .

:RM7x7R4C2 a skos:Concept ;
    skos:broader :RiskMatrix7x7 ;
    skos:definition "Node (row: 4, col: 2) in 7x7 risk matrix with risk level 2, severity VeryLow, and likelihood Moderate"@en ;
    skos:prefLabel "Low Risk"@en ;
    dpv:hasLikelihood :ModerateLikelihood ;
    dpv:hasRiskLevel :LowRisk ;
    dpv:hasSeverity :VeryLowSeverity .

:RM7x7R4C3 a skos:Concept ;
    skos:broader :RiskMatrix7x7 ;
    skos:definition "Node (row: 4, col: 3) in 7x7 risk matrix with risk level 3, severity Low, and likelihood Moderate"@en ;
    skos:prefLabel "Moderate Risk"@en ;
    dpv:hasLikelihood :ModerateLikelihood ;
    dpv:hasRiskLevel :ModerateRisk ;
    dpv:hasSeverity :LowSeverity .

:RM7x7R4C4 a skos:Concept ;
    skos:broader :RiskMatrix7x7 ;
    skos:definition "Node (row: 4, col: 4) in 7x7 risk matrix with risk level 4, severity Moderate, and likelihood Moderate"@en ;
    skos:prefLabel "High Risk"@en ;
    dpv:hasLikelihood :ModerateLikelihood ;
    dpv:hasRiskLevel :HighRisk ;
    dpv:hasSeverity :ModerateSeverity .

:RM7x7R4C5 a skos:Concept ;
    skos:broader :RiskMatrix7x7 ;
    skos:definition "Node (row: 4, col: 5) in 7x7 risk matrix with risk level 4, severity High, and likelihood Moderate"@en ;
    skos:prefLabel "High Risk"@en ;
    dpv:hasLikelihood :ModerateLikelihood ;
    dpv:hasRiskLevel :HighRisk ;
    dpv:hasSeverity :HighSeverity .

:RM7x7R4C6 a skos:Concept ;
    skos:broader :RiskMatrix7x7 ;
    skos:definition "Node (row: 4, col: 6) in 7x7 risk matrix with risk level 5, severity VeryHigh, and likelihood Moderate"@en ;
    skos:prefLabel "Very High Risk"@en ;
    dpv:hasLikelihood :ModerateLikelihood ;
    dpv:hasRiskLevel :VeryHighRisk ;
    dpv:hasSeverity :VeryHighSeverity .

:RM7x7R4C7 a skos:Concept ;
    skos:broader :RiskMatrix7x7 ;
    skos:definition "Node (row: 4, col: 7) in 7x7 risk matrix with risk level 5, severity ExtremelyHigh, and likelihood Moderate"@en ;
    skos:prefLabel "Very High Risk"@en ;
    dpv:hasLikelihood :ModerateLikelihood ;
    dpv:hasRiskLevel :VeryHighRisk ;
    dpv:hasSeverity :ExtremelyHighSeverity .

:RM7x7R5C1 a skos:Concept ;
    skos:broader :RiskMatrix7x7 ;
    skos:definition "Node (row: 5, col: 1) in 7x7 risk matrix with risk level 1, severity ExtremelyLow, and likelihood High"@en ;
    skos:prefLabel "Very Low Risk"@en ;
    dpv:hasLikelihood :HighLikelihood ;
    dpv:hasRiskLevel :VeryLowRisk ;
    dpv:hasSeverity :ExtremelyLowSeverity .

:RM7x7R5C2 a skos:Concept ;
    skos:broader :RiskMatrix7x7 ;
    skos:definition "Node (row: 5, col: 2) in 7x7 risk matrix with risk level 2, severity VeryLow, and likelihood High"@en ;
    skos:prefLabel "Low Risk"@en ;
    dpv:hasLikelihood :HighLikelihood ;
    dpv:hasRiskLevel :LowRisk ;
    dpv:hasSeverity :VeryLowSeverity .

:RM7x7R5C3 a skos:Concept ;
    skos:broader :RiskMatrix7x7 ;
    skos:definition "Node (row: 5, col: 3) in 7x7 risk matrix with risk level 4, severity Low, and likelihood High"@en ;
    skos:prefLabel "High Risk"@en ;
    dpv:hasLikelihood :HighLikelihood ;
    dpv:hasRiskLevel :HighRisk ;
    dpv:hasSeverity :LowSeverity .

:RM7x7R5C4 a skos:Concept ;
    skos:broader :RiskMatrix7x7 ;
    skos:definition "Node (row: 5, col: 4) in 7x7 risk matrix with risk level 4, severity Moderate, and likelihood High"@en ;
    skos:prefLabel "High Risk"@en ;
    dpv:hasLikelihood :HighLikelihood ;
    dpv:hasRiskLevel :HighRisk ;
    dpv:hasSeverity :ModerateSeverity .

:RM7x7R5C5 a skos:Concept ;
    skos:broader :RiskMatrix7x7 ;
    skos:definition "Node (row: 5, col: 5) in 7x7 risk matrix with risk level 5, severity High, and likelihood High"@en ;
    skos:prefLabel "Very High Risk"@en ;
    dpv:hasLikelihood :HighLikelihood ;
    dpv:hasRiskLevel :VeryHighRisk ;
    dpv:hasSeverity :HighSeverity .

:RM7x7R5C6 a skos:Concept ;
    skos:broader :RiskMatrix7x7 ;
    skos:definition "Node (row: 5, col: 6) in 7x7 risk matrix with risk level 5, severity VeryHigh, and likelihood High"@en ;
    skos:prefLabel "Very High Risk"@en ;
    dpv:hasLikelihood :HighLikelihood ;
    dpv:hasRiskLevel :VeryHighRisk ;
    dpv:hasSeverity :VeryHighSeverity .

:RM7x7R5C7 a skos:Concept ;
    skos:broader :RiskMatrix7x7 ;
    skos:definition "Node (row: 5, col: 7) in 7x7 risk matrix with risk level 6, severity ExtremelyHigh, and likelihood High"@en ;
    skos:prefLabel "Extremely High Risk"@en ;
    dpv:hasLikelihood :HighLikelihood ;
    dpv:hasRiskLevel :ExtremelyHighRisk ;
    dpv:hasSeverity :ExtremelyHighSeverity .

:RM7x7R6C1 a skos:Concept ;
    skos:broader :RiskMatrix7x7 ;
    skos:definition "Node (row: 6, col: 1) in 7x7 risk matrix with risk level 1, severity ExtremelyLow, and likelihood VeryHigh"@en ;
    skos:prefLabel "Very Low Risk"@en ;
    dpv:hasLikelihood :VeryHighLikelihood ;
    dpv:hasRiskLevel :VeryLowRisk ;
    dpv:hasSeverity :ExtremelyLowSeverity .

:RM7x7R6C2 a skos:Concept ;
    skos:broader :RiskMatrix7x7 ;
    skos:definition "Node (row: 6, col: 2) in 7x7 risk matrix with risk level 3, severity VeryLow, and likelihood VeryHigh"@en ;
    skos:prefLabel "Moderate Risk"@en ;
    dpv:hasLikelihood :VeryHighLikelihood ;
    dpv:hasRiskLevel :ModerateRisk ;
    dpv:hasSeverity :VeryLowSeverity .

:RM7x7R6C3 a skos:Concept ;
    skos:broader :RiskMatrix7x7 ;
    skos:definition "Node (row: 6, col: 3) in 7x7 risk matrix with risk level 4, severity Low, and likelihood VeryHigh"@en ;
    skos:prefLabel "High Risk"@en ;
    dpv:hasLikelihood :VeryHighLikelihood ;
    dpv:hasRiskLevel :HighRisk ;
    dpv:hasSeverity :LowSeverity .

:RM7x7R6C4 a skos:Concept ;
    skos:broader :RiskMatrix7x7 ;
    skos:definition "Node (row: 6, col: 4) in 7x7 risk matrix with risk level 5, severity Moderate, and likelihood VeryHigh"@en ;
    skos:prefLabel "Very High Risk"@en ;
    dpv:hasLikelihood :VeryHighLikelihood ;
    dpv:hasRiskLevel :VeryHighRisk ;
    dpv:hasSeverity :ModerateSeverity .

:RM7x7R6C5 a skos:Concept ;
    skos:broader :RiskMatrix7x7 ;
    skos:definition "Node (row: 6, col: 5) in 7x7 risk matrix with risk level 6, severity High, and likelihood VeryHigh"@en ;
    skos:prefLabel "Extremely High Risk"@en ;
    dpv:hasLikelihood :VeryHighLikelihood ;
    dpv:hasRiskLevel :ExtremelyHighRisk ;
    dpv:hasSeverity :HighSeverity .

:RM7x7R6C6 a skos:Concept ;
    skos:broader :RiskMatrix7x7 ;
    skos:definition "Node (row: 6, col: 6) in 7x7 risk matrix with risk level 6, severity VeryHigh, and likelihood VeryHigh"@en ;
    skos:prefLabel "Extremely High Risk"@en ;
    dpv:hasLikelihood :VeryHighLikelihood ;
    dpv:hasRiskLevel :ExtremelyHighRisk ;
    dpv:hasSeverity :VeryHighSeverity .

:RM7x7R6C7 a skos:Concept ;
    skos:broader :RiskMatrix7x7 ;
    skos:definition "Node (row: 6, col: 7) in 7x7 risk matrix with risk level 6, severity ExtremelyHigh, and likelihood VeryHigh"@en ;
    skos:prefLabel "Extremely High Risk"@en ;
    dpv:hasLikelihood :VeryHighLikelihood ;
    dpv:hasRiskLevel :ExtremelyHighRisk ;
    dpv:hasSeverity :ExtremelyHighSeverity .

:RM7x7R7C1 a skos:Concept ;
    skos:broader :RiskMatrix7x7 ;
    skos:definition "Node (row: 7, col: 1) in 7x7 risk matrix with risk level 2, severity ExtremelyLow, and likelihood ExtremelyHigh"@en ;
    skos:prefLabel "Low Risk"@en ;
    dpv:hasLikelihood :ExtremelyHighLikelihood ;
    dpv:hasRiskLevel :LowRisk ;
    dpv:hasSeverity :ExtremelyLowSeverity .

:RM7x7R7C2 a skos:Concept ;
    skos:broader :RiskMatrix7x7 ;
    skos:definition "Node (row: 7, col: 2) in 7x7 risk matrix with risk level 3, severity VeryLow, and likelihood ExtremelyHigh"@en ;
    skos:prefLabel "Moderate Risk"@en ;
    dpv:hasLikelihood :ExtremelyHighLikelihood ;
    dpv:hasRiskLevel :ModerateRisk ;
    dpv:hasSeverity :VeryLowSeverity .

:RM7x7R7C3 a skos:Concept ;
    skos:broader :RiskMatrix7x7 ;
    skos:definition "Node (row: 7, col: 3) in 7x7 risk matrix with risk level 5, severity Low, and likelihood ExtremelyHigh"@en ;
    skos:prefLabel "Very High Risk"@en ;
    dpv:hasLikelihood :ExtremelyHighLikelihood ;
    dpv:hasRiskLevel :VeryHighRisk ;
    dpv:hasSeverity :LowSeverity .

:RM7x7R7C4 a skos:Concept ;
    skos:broader :RiskMatrix7x7 ;
    skos:definition "Node (row: 7, col: 4) in 7x7 risk matrix with risk level 5, severity Moderate, and likelihood ExtremelyHigh"@en ;
    skos:prefLabel "Very High Risk"@en ;
    dpv:hasLikelihood :ExtremelyHighLikelihood ;
    dpv:hasRiskLevel :VeryHighRisk ;
    dpv:hasSeverity :ModerateSeverity .

:RM7x7R7C5 a skos:Concept ;
    skos:broader :RiskMatrix7x7 ;
    skos:definition "Node (row: 7, col: 5) in 7x7 risk matrix with risk level 6, severity High, and likelihood ExtremelyHigh"@en ;
    skos:prefLabel "Extremely High Risk"@en ;
    dpv:hasLikelihood :ExtremelyHighLikelihood ;
    dpv:hasRiskLevel :ExtremelyHighRisk ;
    dpv:hasSeverity :HighSeverity .

:RM7x7R7C6 a skos:Concept ;
    skos:broader :RiskMatrix7x7 ;
    skos:definition "Node (row: 7, col: 6) in 7x7 risk matrix with risk level 6, severity VeryHigh, and likelihood ExtremelyHigh"@en ;
    skos:prefLabel "Extremely High Risk"@en ;
    dpv:hasLikelihood :ExtremelyHighLikelihood ;
    dpv:hasRiskLevel :ExtremelyHighRisk ;
    dpv:hasSeverity :VeryHighSeverity .

:RM7x7R7C7 a skos:Concept ;
    skos:broader :RiskMatrix7x7 ;
    skos:definition "Node (row: 7, col: 7) in 7x7 risk matrix with risk level 6, severity ExtremelyHigh, and likelihood ExtremelyHigh"@en ;
    skos:prefLabel "Extremely High Risk"@en ;
    dpv:hasLikelihood :ExtremelyHighLikelihood ;
    dpv:hasRiskLevel :ExtremelyHighRisk ;
    dpv:hasSeverity :ExtremelyHighSeverity .
