@prefix : <https://w3id.org/dpv/risk/matrix#> .

:RiskMatrixLevel a skos:Concept ;
    skos:prefLabel "Risk Matrix Level"@en ;
    skos:definition "Risk Level as expressed as a combination of Severity and Likelihood within a Risk Matrix"@en ;
    skos:broader :RiskLevel .

:RiskMatrix3x3 a skos:Concept ;
    skos:prefLabel "Risk Matrix 3x3"@en ;
    skos:definition "A Risk Matrix with 3 Risk Levels, 3 Severity levels, and 3 Likelihood levels"@en ;
    skos:broader :RiskMatrix .
:RiskMatrix5x5 a skos:Concept ;
    skos:prefLabel "Risk Matrix 5x5"@en ;
    skos:definition "A Risk Matrix with 3 Risk Levels, 3 Severity levels, and 3 Likelihood levels"@en ;
    skos:broader :RiskMatrix .
:RiskMatrix7x7 a skos:Concept ;
    skos:prefLabel "Risk Matrix 7x7"@en ;
    skos:definition "A Risk Matrix with 3 Risk Levels, 3 Severity levels, and 3 Likelihood levels"@en ;
    skos:broader :RiskMatrix .

# e.g. of how to create a risk matrix for use
:RM3x3N1 a skos:Concept, :RiskLevel, :RiskMatrixLevel ;
    skos:prefLabel "Low Risk"@en ;
    :associatedRiskLevel :LowRisk ;
    :associatedRiskSeverity :LowSeverity ;
    :associatedRiskLikelihood :LowLikelihood ;
    skos:broader :RiskMatrix3x3 .